% The proof is discussed in the appendix A.4.1. %~\ref{proof:slowOnlineSensitivityBound}. 
% \begin{proof}{\label{proof:slowOnlineSensitivityBound}}
%  We define the online sensitivity scores $\tilde{s}_{i}$ for each point $i$ as follows,
%   \allowdisplaybreaks
%   \begin{eqnarray*}
%   \tilde{s}_{i} &=& \sup_{\{\*x\mid\|\*x\|=1\}}\frac{|\*a_{i}^{T}\*x|^{p}}{\|\*A_{i}\*x\|_{p}^{p}} = \sup_{\{\*x\mid\|\*x\|=1\}}\frac{|\*a_{i}^{T}\*x|^{\lfloor p/2 \rfloor}|\*a_{i}^{T}\*x|^{\lceil p/2 \rceil}}{\|\*A_{i}\*x\|_{p}^{p}} = \sup_{\{\*x,\grave{\*x},\acute{\*x}\mid\|\*x\|=1\}}\frac{|\grave{\*x}^{T}\grave{\*a}_{i}\acute{\*a}_{i}^{T}\acute{\*x}|}{\|\*A_{i}\*x\|_{p}^{p}} \\
%   &\stackrel{(i)}=& \sup_{\{\*x,\grave{\*z},\acute{\*z}\mid\|\*x\|=1\}}\frac{|\grave{\*z}^{T}\grave{\*u}_{i}\acute{\*u}_{i}^{T}\acute{\*z}|\cdot(\|\grave{\*z}\|\|\acute{\*z}\|)}{\|\*A_{i}\*x\|_{p}^{p}\cdot(\|\grave{\*z}\|\|\acute{\*z}\|)} \\
%   &\stackrel{(ii)}\leq& \sup_{\{\*x,\grave{\*y},\acute{\*y},\grave{\*z},\acute{\*z}\mid\|\*x\|=1\}}\frac{|\grave{\*y}^{T}\grave{\*u}_{i}\acute{\*u}_{i}^{T}\acute{\*y}|\cdot(\|\grave{\*z}\|\|\acute{\*z}\|)}{\|\*A_{i}\*x\|_{p}^{p}} \\
%   &\stackrel{(iii)}=& \sup_{\{\*x,\grave{\*y},\acute{\*y},\grave{\*z},\acute{\*z}\mid\|\*x\|=1\}}\frac{|\grave{\*y}^{T}\grave{\*u}_{i}\acute{\*u}_{i}^{T}\acute{\*y}|\cdot\|\grave{\*z}\acute{\*z}^{T}\|}{\|\*A_{i}\*x\|_{p}^{p}} \\
%   &\stackrel{(iv)}=& \sup_{\{\*x,\grave{\*y},\acute{\*y}\mid\|\*x\|=1\}}\frac{|\grave{\*y}^{T}\grave{\*u}_{i}\acute{\*u}_{i}^{T}\acute{\*y}|\cdot\|\grave{\*\Sigma}_{i}\grave{\*V}_{i}^{T}\grave{\*x}\acute{\*x}^{T}\acute{\*V}_{i}\acute{\*\Sigma}_{i}\|}{\|\*A_{i}\*x\|_{p}^{p}} \\
%   &\stackrel{(v)}=& \sup_{\{\*x,\grave{\*y},\acute{\*y}\mid\|\*x\|=1\}}\frac{|\grave{\*y}^{T}\grave{\*u}_{i}\acute{\*u}_{i}^{T}\acute{\*y}| \cdot\|\grave{\*U}_{i}\grave{\*\Sigma}_{i}\grave{\*V}_{i}^{T}\grave{\*x}\acute{\*x}^{T}\acute{\*V}_{i}\acute{\*\Sigma}_{i}\acute{\*U}_{i}^{T}\|}{\|\*A_{i}\*x\|_{p}^{p}} = \sup_{\{\*x,\grave{\*y},\acute{\*y}\mid\|\*x\|=1\}}\frac{|\grave{\*y}^{T}\grave{\*u}_{i}\acute{\*u}_{i}^{T}\acute{\*y}|\cdot\|\grave{\*A}_{i}\grave{\*x}\acute{\*x}^{T}\acute{\*A}_{i}^{T}\|}{\|\*A_{i}\*x\|_{p}^{p}} \\
%   &\stackrel{(vi)}=& \sup_{\{\*x,\grave{\*y},\acute{\*y}\mid\|\*x\|=1\}}\frac{|\grave{\*y}^{T}\grave{\*u}_{i}\acute{\*u}_{i}^{T}\acute{\*y}|\cdot\mbox{Trace}(\grave{\*A}_{i}\grave{\*x}\acute{\*x}^{T}\acute{\*A}_{i}^{T})}{\|\*A_{i}\*x\|_{p}^{p}} \leq \sup_{\{\*x,\grave{\*y},\acute{\*y}\mid\|\*x\|=1\}}\frac{|\grave{\*y}^{T}\grave{\*u}_{i}\acute{\*u}_{i}^{T}\acute{\*y}|\cdot\big(\sum_{j=1}^{i}|\grave{\*x}^{T}\grave{\*a}_{j}\acute{\*a}_{j}^{T}\acute{\*x}|\big)}{\|\*A_{i}\*x\|_{p}^{p}} \\
%   &=& \sup_{\{\*x,\grave{\*y},\acute{\*y}\mid\|\*x\|=1\}}\frac{|\grave{\*y}^{T}\grave{\*u}_{i}\acute{\*u}_{i}^{T}\acute{\*y}|\cdot\|\*A_{i}\*x\|_{p}^{p}}{\|\*A_{i}\*x\|_{p}^{p}} = \sup_{\{\grave{\*y},\acute{\*y}\mid\|\*x\|=1\}}|\grave{\*y}^{T}\grave{\*u}_{i}\acute{\*u}_{i}^{T}\acute{\*y}| = \|\grave{\*u}_{i}\|\cdot\|\acute{\*u}_{i}\|
%  \end{eqnarray*}
%  Let $\grave{\*A}$ be the matrix where its $j^{th}$ row $\grave{\*a}_{j} = \*a \otimes^{d^{\lfloor p/2 \rfloor}} \in \~R^{d^{\lfloor p/2 \rfloor}}$ and $\acute{\*A}$ be the matrix where its $j^{th}$ row $\acute{\*a}_{j} = \*a \otimes^{d^{\lceil p/2 \rceil}} \in \~R^{d^{\lceil p/2 \rceil}}$. Further let $\grave{\*A}_{i}$ and $\acute{\*A}_{i}$ are the corresponding matrices $\*A_{i} \in \~R^{i \times d}$ which represents first $i$ streaming rows. We define $[\grave{\*U}_{i},\grave{\*\Sigma}_{i},\grave{\*V}_{i}] = \mbox{svd}(\grave{\*A}_{i})$ such that $\grave{\*a}_{i}^{T} = \grave{\*u}_{i}^{T}\grave{\*\Sigma}_{i}\grave{\*V}_{i}^{T}$ and $[\acute{\*U}_{i},\acute{\*\Sigma}_{i},\acute{\*V}_{i}] = \mbox{svd}(\acute{\*A}_{i})$ such that $\acute{\*a}_{i}^{T} = \acute{\*u}_{i}^{T}\acute{\*\Sigma}_{i}\acute{\*V}_{i}^{T}$. Now for a fixed $\*x \in \~R^{d}$ its corresponding $\grave{\*x}$ and $\acute{\*x}$ are also fixed in their corresponding higher dimensions. Here $\grave{\*\Sigma}_{i}\grave{\*V}_{i}^{T}\grave{\*x}=\grave{\*z}$ and $\acute{\*\Sigma}_{i}\acute{\*V}_{i}^{T}\acute{\*x}=\acute{\*z}$ from which we define unit vectors $\grave{\*y} = \grave{\*z}/\|\grave{\*y}\|$ and $\acute{\*y} = \acute{\*z}/\|\acute{\*z}\|$.

%  Now The equality (i) is by change of variable where $\grave{\*z}$ and $\acute{\*z}$ are still function of $\*x$ so $\sup$ is still over $\*x$. The (ii) inequality is due to the $\sup$ is over $\grave{\*y}$ and $\acute{\*y}$. Note that $\forall \*x, \exists \grave{\*y}$ and $\exists \acute{\*y}$. The (iii) equality follows by the fact that for any two vector $\*a$ and $\*b$ we know that $\|\*a\|\|\*b\| = \|\*a\*b^{T}\|_{F} = \|\*a\*b^{T}\|$. The (iv) equality is directly by substituting $\grave{\*z}$ and $\acute{\*z}$. The (v) equality follows by adding scale invariant orthonormal column basis $\grave{\*U}$ and $\acute{\*U}$. The (vi) is equality is by the fact that the matrix $\grave{\*A}\grave{\*x}\acute{\*x}^{T}\acute{\*A}^{T}$ is a rank-1 matrix, so we know that the spectral norm is equal to the Frobenius norm of the matrix which is further equal to the trace of the matrix. 

%   Another approach analysis
%   \begin{eqnarray*}
%   \tilde{s}_{i} &=& \sup_{\{\*x\mid\|\*x\|=1\}}\frac{|\*a_{i}^{T}\*x|^{p}}{\|\*A_{i}\*x\|_{p}^{p}} = \sup_{\{\*x\mid\|\*x\|=1\}}\frac{|\*a_{i}^{T}\*x|^{\lfloor p/2 \rfloor}|\*a_{i}^{T}\*x|^{\lceil p/2 \rceil}}{\|\*A_{i}\*x\|_{p}^{p}} = \sup_{\{\grave{\*x},\acute{\*x}\mid\|\*x\|=1\}}\frac{|\grave{\*x}^{T}\grave{\*a}_{i}\acute{\*a}_{i}^{T}\acute{\*x}|}{\sum_{j=1}^{i}|\grave{\*x}^{T}\grave{\*a}_{j}\acute{\*a}_{j}^{T}\acute{\*x}|} \\
%   &\leq& \sup_{\{\grave{\*x},\acute{\*x}\mid\|\*x\|=1\}}\frac{|\grave{\*x}^{T}\grave{\*a}_{i}\acute{\*a}_{i}^{T}\acute{\*x}|}{|\grave{\*x}^{T}\grave{\*A}_{i}^{T}\acute{\*A}_{i}\acute{\*x}|}  =  \sup_{\{\grave{\*x},\acute{\*x}\mid\|\*x\|=1\}}|\grave{\*a}_{i}^{T}\grave{\*x}||\acute{\*x}^{T}\acute{\*A}_{i}^{T}\grave{\*A}_{i}\grave{\*x}|^{\dagger}|\acute{\*x}^{T}\acute{\*a}_{i}| \\
%   &=& \sup_{\{\grave{\*x},\acute{\*x}\mid\|\*x\|=1\}}|\grave{\*a}_{i}^{T}\grave{\*x}||\grave{\*A}_{i}\grave{\*x}|^{\dagger}|\acute{\*x}^{T}\acute{\*A}_{i}^{T}|^{\dagger}|\acute{\*x}^{T}\acute{\*a}_{i}| \leq \sup_{\{\grave{\*x},\acute{\*x}\mid\|\*x\|=1\}}\|\grave{\*a}_{i}^{T}\grave{\*x}\grave{\*x}^{\dagger}\grave{\*A}_{i}^{\dagger}\| \|\acute{\*a}_{i}^{T}\acute{\*x}\acute{\*x}^{\dagger}\acute{\*A}_{i}^{\dagger}\| \\
%   &\leq& \|\grave{\*a}_{i}^{T}\grave{\*A}_{i}^{\dagger}\| \|\acute{\*a}_{i}^{T}\acute{\*A}_{i}^{\dagger}\| = \|\grave{\*u}_{i}\|\cdot\|\acute{\*u}_{i}\|
% %   &\stackrel{(v)}=& \sup_{\{\*x,\grave{\*y},\acute{\*y}\mid\|\*x\|=1\}}\frac{|\grave{\*y}^{T}\grave{\*u}_{i}\acute{\*u}_{i}^{T}\acute{\*y}| \cdot\|\grave{\*U}_{i}\grave{\*\Sigma}_{i}\grave{\*V}_{i}^{T}\grave{\*x}\acute{\*x}^{T}\acute{\*V}_{i}\acute{\*\Sigma}_{i}\acute{\*U}_{i}^{T}\|}{\|\*A_{i}\*x\|_{p}^{p}} = \sup_{\{\*x,\grave{\*y},\acute{\*y}\mid\|\*x\|=1\}}\frac{|\grave{\*y}^{T}\grave{\*u}_{i}\acute{\*u}_{i}^{T}\acute{\*y}|\cdot\|\grave{\*A}_{i}\grave{\*x}\acute{\*x}^{T}\acute{\*A}_{i}^{T}\|}{\|\*A_{i}\*x\|_{p}^{p}} \\
% %   &\stackrel{(vi)}=& \sup_{\{\*x,\grave{\*y},\acute{\*y}\mid\|\*x\|=1\}}\frac{|\grave{\*y}^{T}\grave{\*u}_{i}\acute{\*u}_{i}^{T}\acute{\*y}|\cdot\mbox{Trace}(\grave{\*A}_{i}\grave{\*x}\acute{\*x}^{T}\acute{\*A}_{i}^{T})}{\|\*A_{i}\*x\|_{p}^{p}} \leq \sup_{\{\*x,\grave{\*y},\acute{\*y}\mid\|\*x\|=1\}}\frac{|\grave{\*y}^{T}\grave{\*u}_{i}\acute{\*u}_{i}^{T}\acute{\*y}|\cdot\big(\sum_{j=1}^{i}|\grave{\*x}^{T}\grave{\*a}_{j}\acute{\*a}_{j}^{T}\acute{\*x}|\big)}{\|\*A_{i}\*x\|_{p}^{p}} \\
% %   &=& \sup_{\{\*x,\grave{\*y},\acute{\*y}\mid\|\*x\|=1\}}\frac{|\grave{\*y}^{T}\grave{\*u}_{i}\acute{\*u}_{i}^{T}\acute{\*y}|\cdot\|\*A_{i}\*x\|_{p}^{p}}{\|\*A_{i}\*x\|_{p}^{p}} = \sup_{\{\grave{\*y},\acute{\*y}\mid\|\*x\|=1\}}|\grave{\*y}^{T}\grave{\*u}_{i}\acute{\*u}_{i}^{T}\acute{\*y}| = \|\grave{\*u}_{i}\|\cdot\|\acute{\*u}_{i}\|
%  \end{eqnarray*}
% % 
% % 
%  Note that for even value $p$ we get $\tilde{s}_{i} \leq \|\hat{\*u}_{i}\|^{2}$ as by lemma \ref{lemma:kernel} we get $\grave{\*u}_{i} = \acute{\*u}_{i} = \hat{\*u}_{i}$. In fact this is true because for even $p$ we have $\lfloor p/2 \rfloor = \lceil p/2 \rceil$.
% \end{proof}
